coq/default.nix
@@ -1,8 +1,17 @@
 { pkgs ? (import <nixpkgs> {})
 }:
 
+let
+  ocamlInit = pkgs.writeText "ocamlinit" ''
+    #use "topfind";;
+  '';
+in
 pkgs.mkShell {
-  buildInputs = [ pkgs.coq ];
+  buildInputs = [ pkgs.coq
+                  pkgs.coq.ocaml
+                  pkgs.coq.ocamlPackages.utop ];
   shellHook = ''
+    alias ocaml="ocaml -init ${ocamlInit}"
+    alias utop="utop -init ${ocamlInit}"
   '';
 }
